Generated files (change of spec)

src/FcEtt/ett_inf.v
@@ -50,6 +50,18 @@ Definition appflag_mutrec :=
   fun H1 H2 H3 =>
   appflag_rec' H1 H2 H3.
 
+Scheme F_ind' := Induction for F Sort Prop.
+
+Definition F_mutind :=
+  fun H1 H2 H3 =>
+  F_ind' H1 H2 H3.
+
+Scheme F_rec' := Induction for F Sort Set.
+
+Definition F_mutrec :=
+  fun H1 H2 H3 =>
+  F_rec' H1 H2 H3.
+
 Scheme App_ind' := Induction for App Sort Prop.
 
 Definition App_mutind :=
@@ -80,11 +92,11 @@ Scheme tm_ind' := Induction for tm Sort Prop
   with constraint_ind' := Induction for constraint Sort Prop.
 
 Definition tm_brs_co_constraint_mutind :=
-  fun H1 H2 H3 H4 H5 H6 H7 H8 H9 H10 H11 H12 H13 H14 H15 H16 H17 H18 H19 H20 H21 H22 H23 H24 H25 H26 H27 H28 H29 H30 H31 H32 H33 H34 H35 H36 H37 H38 H39 H40 H41 H42 H43 H44 H45 H46 H47 H48 H49 H50 H51 H52 H53 =>
-  (conj (tm_ind' H1 H2 H3 H4 H5 H6 H7 H8 H9 H10 H11 H12 H13 H14 H15 H16 H17 H18 H19 H20 H21 H22 H23 H24 H25 H26 H27 H28 H29 H30 H31 H32 H33 H34 H35 H36 H37 H38 H39 H40 H41 H42 H43 H44 H45 H46 H47 H48 H49 H50 H51 H52 H53)
-  ((conj (brs_ind' H1 H2 H3 H4 H5 H6 H7 H8 H9 H10 H11 H12 H13 H14 H15 H16 H17 H18 H19 H20 H21 H22 H23 H24 H25 H26 H27 H28 H29 H30 H31 H32 H33 H34 H35 H36 H37 H38 H39 H40 H41 H42 H43 H44 H45 H46 H47 H48 H49 H50 H51 H52 H53)
-  ((conj (co_ind' H1 H2 H3 H4 H5 H6 H7 H8 H9 H10 H11 H12 H13 H14 H15 H16 H17 H18 H19 H20 H21 H22 H23 H24 H25 H26 H27 H28 H29 H30 H31 H32 H33 H34 H35 H36 H37 H38 H39 H40 H41 H42 H43 H44 H45 H46 H47 H48 H49 H50 H51 H52 H53)
-  (constraint_ind' H1 H2 H3 H4 H5 H6 H7 H8 H9 H10 H11 H12 H13 H14 H15 H16 H17 H18 H19 H20 H21 H22 H23 H24 H25 H26 H27 H28 H29 H30 H31 H32 H33 H34 H35 H36 H37 H38 H39 H40 H41 H42 H43 H44 H45 H46 H47 H48 H49 H50 H51 H52 H53)))))).
+  fun H1 H2 H3 H4 H5 H6 H7 H8 H9 H10 H11 H12 H13 H14 H15 H16 H17 H18 H19 H20 H21 H22 H23 H24 H25 H26 H27 H28 H29 H30 H31 H32 H33 H34 H35 H36 H37 H38 H39 H40 H41 H42 H43 H44 H45 H46 H47 H48 H49 H50 H51 H52 =>
+  (conj (tm_ind' H1 H2 H3 H4 H5 H6 H7 H8 H9 H10 H11 H12 H13 H14 H15 H16 H17 H18 H19 H20 H21 H22 H23 H24 H25 H26 H27 H28 H29 H30 H31 H32 H33 H34 H35 H36 H37 H38 H39 H40 H41 H42 H43 H44 H45 H46 H47 H48 H49 H50 H51 H52)
+  ((conj (brs_ind' H1 H2 H3 H4 H5 H6 H7 H8 H9 H10 H11 H12 H13 H14 H15 H16 H17 H18 H19 H20 H21 H22 H23 H24 H25 H26 H27 H28 H29 H30 H31 H32 H33 H34 H35 H36 H37 H38 H39 H40 H41 H42 H43 H44 H45 H46 H47 H48 H49 H50 H51 H52)
+  ((conj (co_ind' H1 H2 H3 H4 H5 H6 H7 H8 H9 H10 H11 H12 H13 H14 H15 H16 H17 H18 H19 H20 H21 H22 H23 H24 H25 H26 H27 H28 H29 H30 H31 H32 H33 H34 H35 H36 H37 H38 H39 H40 H41 H42 H43 H44 H45 H46 H47 H48 H49 H50 H51 H52)
+  (constraint_ind' H1 H2 H3 H4 H5 H6 H7 H8 H9 H10 H11 H12 H13 H14 H15 H16 H17 H18 H19 H20 H21 H22 H23 H24 H25 H26 H27 H28 H29 H30 H31 H32 H33 H34 H35 H36 H37 H38 H39 H40 H41 H42 H43 H44 H45 H46 H47 H48 H49 H50 H51 H52)))))).
 
 Scheme tm_rec' := Induction for tm Sort Set
   with brs_rec' := Induction for brs Sort Set
@@ -92,11 +104,11 @@ Scheme tm_rec' := Induction for tm Sort Set
   with constraint_rec' := Induction for constraint Sort Set.
 
 Definition tm_brs_co_constraint_mutrec :=
-  fun H1 H2 H3 H4 H5 H6 H7 H8 H9 H10 H11 H12 H13 H14 H15 H16 H17 H18 H19 H20 H21 H22 H23 H24 H25 H26 H27 H28 H29 H30 H31 H32 H33 H34 H35 H36 H37 H38 H39 H40 H41 H42 H43 H44 H45 H46 H47 H48 H49 H50 H51 H52 H53 =>
-  (pair ((pair ((pair (tm_rec' H1 H2 H3 H4 H5 H6 H7 H8 H9 H10 H11 H12 H13 H14 H15 H16 H17 H18 H19 H20 H21 H22 H23 H24 H25 H26 H27 H28 H29 H30 H31 H32 H33 H34 H35 H36 H37 H38 H39 H40 H41 H42 H43 H44 H45 H46 H47 H48 H49 H50 H51 H52 H53)
-  (brs_rec' H1 H2 H3 H4 H5 H6 H7 H8 H9 H10 H11 H12 H13 H14 H15 H16 H17 H18 H19 H20 H21 H22 H23 H24 H25 H26 H27 H28 H29 H30 H31 H32 H33 H34 H35 H36 H37 H38 H39 H40 H41 H42 H43 H44 H45 H46 H47 H48 H49 H50 H51 H52 H53)))
-  (co_rec' H1 H2 H3 H4 H5 H6 H7 H8 H9 H10 H11 H12 H13 H14 H15 H16 H17 H18 H19 H20 H21 H22 H23 H24 H25 H26 H27 H28 H29 H30 H31 H32 H33 H34 H35 H36 H37 H38 H39 H40 H41 H42 H43 H44 H45 H46 H47 H48 H49 H50 H51 H52 H53)))
-  (constraint_rec' H1 H2 H3 H4 H5 H6 H7 H8 H9 H10 H11 H12 H13 H14 H15 H16 H17 H18 H19 H20 H21 H22 H23 H24 H25 H26 H27 H28 H29 H30 H31 H32 H33 H34 H35 H36 H37 H38 H39 H40 H41 H42 H43 H44 H45 H46 H47 H48 H49 H50 H51 H52 H53)).
+  fun H1 H2 H3 H4 H5 H6 H7 H8 H9 H10 H11 H12 H13 H14 H15 H16 H17 H18 H19 H20 H21 H22 H23 H24 H25 H26 H27 H28 H29 H30 H31 H32 H33 H34 H35 H36 H37 H38 H39 H40 H41 H42 H43 H44 H45 H46 H47 H48 H49 H50 H51 H52 =>
+  (pair ((pair ((pair (tm_rec' H1 H2 H3 H4 H5 H6 H7 H8 H9 H10 H11 H12 H13 H14 H15 H16 H17 H18 H19 H20 H21 H22 H23 H24 H25 H26 H27 H28 H29 H30 H31 H32 H33 H34 H35 H36 H37 H38 H39 H40 H41 H42 H43 H44 H45 H46 H47 H48 H49 H50 H51 H52)
+  (brs_rec' H1 H2 H3 H4 H5 H6 H7 H8 H9 H10 H11 H12 H13 H14 H15 H16 H17 H18 H19 H20 H21 H22 H23 H24 H25 H26 H27 H28 H29 H30 H31 H32 H33 H34 H35 H36 H37 H38 H39 H40 H41 H42 H43 H44 H45 H46 H47 H48 H49 H50 H51 H52)))
+  (co_rec' H1 H2 H3 H4 H5 H6 H7 H8 H9 H10 H11 H12 H13 H14 H15 H16 H17 H18 H19 H20 H21 H22 H23 H24 H25 H26 H27 H28 H29 H30 H31 H32 H33 H34 H35 H36 H37 H38 H39 H40 H41 H42 H43 H44 H45 H46 H47 H48 H49 H50 H51 H52)))
+  (constraint_rec' H1 H2 H3 H4 H5 H6 H7 H8 H9 H10 H11 H12 H13 H14 H15 H16 H17 H18 H19 H20 H21 H22 H23 H24 H25 H26 H27 H28 H29 H30 H31 H32 H33 H34 H35 H36 H37 H38 H39 H40 H41 H42 H43 H44 H45 H46 H47 H48 H49 H50 H51 H52)).
 
 
 (* *********************************************************************** *)
@@ -104,7 +116,6 @@ Definition tm_brs_co_constraint_mutrec :=
 
 Fixpoint close_tm_wrt_tm_rec (n1 : nat) (x1 : tmvar) (a1 : tm) {struct a1} : tm :=
   match a1 with
-    | a_Star => a_Star
     | a_Var_f x2 => if (x1 == x2) then (a_Var_b n1) else (a_Var_f x2)
     | a_Var_b n2 => if (lt_ge_dec n2 n1) then (a_Var_b n2) else (a_Var_b (S n2))
     | a_Abs rho1 A1 b1 => a_Abs rho1 (close_tm_wrt_tm_rec n1 x1 A1) (close_tm_wrt_tm_rec (S n1) x1 b1)
@@ -169,7 +180,6 @@ with close_constraint_wrt_tm_rec (n1 : nat) (x1 : tmvar) (phi1 : constraint) {st
 
 Fixpoint close_tm_wrt_co_rec (n1 : nat) (c1 : covar) (a1 : tm) {struct a1} : tm :=
   match a1 with
-    | a_Star => a_Star
     | a_Var_f x1 => a_Var_f x1
     | a_Var_b n2 => a_Var_b n2
     | a_Abs rho1 A1 b1 => a_Abs rho1 (close_tm_wrt_co_rec n1 c1 A1) (close_tm_wrt_co_rec n1 c1 b1)
@@ -270,6 +280,12 @@ Fixpoint size_appflag (nu1 : appflag) {struct nu1} : nat :=
     | Rho rho1 => 1 + (size_relflag rho1)
   end.
 
+Fixpoint size_F (F1 : F) {struct F1} : nat :=
+  match F1 with
+    | f_Star => 1
+    | f_Const T1 => 1
+  end.
+
 Fixpoint size_App (App1 : App) {struct App1} : nat :=
   match App1 with
     | A_Tm nu1 => 1 + (size_appflag nu1)
@@ -284,7 +300,6 @@ Fixpoint size_Apps (Apps1 : Apps) {struct Apps1} : nat :=
 
 Fixpoint size_tm (a1 : tm) {struct a1} : nat :=
   match a1 with
-    | a_Star => 1
     | a_Var_f x1 => 1
     | a_Var_b n1 => 1
     | a_Abs rho1 A1 b1 => 1 + (size_relflag rho1) + (size_tm A1) + (size_tm b1)
@@ -296,9 +311,9 @@ Fixpoint size_tm (a1 : tm) {struct a1} : nat :=
     | a_CApp a2 g1 => 1 + (size_tm a2) + (size_co g1)
     | a_CPi phi1 B1 => 1 + (size_constraint phi1) + (size_tm B1)
     | a_Conv a2 R1 g1 => 1 + (size_tm a2) + (size_role R1) + (size_co g1)
-    | a_Fam F1 => 1
+    | a_Fam F1 => 1 + (size_F F1)
     | a_Bullet => 1
-    | a_Pattern R1 a2 F1 Apps1 b1 b2 => 1 + (size_role R1) + (size_tm a2) + (size_Apps Apps1) + (size_tm b1) + (size_tm b2)
+    | a_Pattern R1 a2 F1 Apps1 b1 b2 => 1 + (size_role R1) + (size_tm a2) + (size_F F1) + (size_Apps Apps1) + (size_tm b1) + (size_tm b2)
     | a_DataCon K1 => 1
     | a_Case a2 brs1 => 1 + (size_tm a2) + (size_brs brs1)
     | a_Sub R1 a2 => 1 + (size_role R1) + (size_tm a2)
@@ -354,8 +369,6 @@ with size_constraint (phi1 : constraint) {struct phi1} : nat :=
 (** These define only an upper bound, not a strict upper bound. *)
 
 Inductive degree_tm_wrt_tm : nat -> tm -> Prop :=
-  | degree_wrt_tm_a_Star : forall n1,
-    degree_tm_wrt_tm n1 (a_Star)
   | degree_wrt_tm_a_Var_f : forall n1 x1,
     degree_tm_wrt_tm n1 (a_Var_f x1)
   | degree_wrt_tm_a_Var_b : forall n1 n2,
@@ -535,8 +548,6 @@ with degree_constraint_wrt_tm : nat -> constraint -> Prop :=
     degree_constraint_wrt_tm n1 (Eq a1 b1 A1 R1).
 
 Inductive degree_tm_wrt_co : nat -> tm -> Prop :=
-  | degree_wrt_co_a_Star : forall n1,
-    degree_tm_wrt_co n1 (a_Star)
   | degree_wrt_co_a_Var_f : forall n1 x1,
     degree_tm_wrt_co n1 (a_Var_f x1)
   | degree_wrt_co_a_Var_b : forall n1 n2,
@@ -721,11 +732,11 @@ Scheme degree_tm_wrt_tm_ind' := Induction for degree_tm_wrt_tm Sort Prop
   with degree_constraint_wrt_tm_ind' := Induction for degree_constraint_wrt_tm Sort Prop.
 
 Definition degree_tm_wrt_tm_degree_brs_wrt_tm_degree_co_wrt_tm_degree_constraint_wrt_tm_mutind :=
-  fun H1 H2 H3 H4 H5 H6 H7 H8 H9 H10 H11 H12 H13 H14 H15 H16 H17 H18 H19 H20 H21 H22 H23 H24 H25 H26 H27 H28 H29 H30 H31 H32 H33 H34 H35 H36 H37 H38 H39 H40 H41 H42 H43 H44 H45 H46 H47 H48 H49 H50 H51 H52 H53 =>
-  (conj (degree_tm_wrt_tm_ind' H1 H2 H3 H4 H5 H6 H7 H8 H9 H10 H11 H12 H13 H14 H15 H16 H17 H18 H19 H20 H21 H22 H23 H24 H25 H26 H27 H28 H29 H30 H31 H32 H33 H34 H35 H36 H37 H38 H39 H40 H41 H42 H43 H44 H45 H46 H47 H48 H49 H50 H51 H52 H53)
-  ((conj (degree_brs_wrt_tm_ind' H1 H2 H3 H4 H5 H6 H7 H8 H9 H10 H11 H12 H13 H14 H15 H16 H17 H18 H19 H20 H21 H22 H23 H24 H25 H26 H27 H28 H29 H30 H31 H32 H33 H34 H35 H36 H37 H38 H39 H40 H41 H42 H43 H44 H45 H46 H47 H48 H49 H50 H51 H52 H53)
-  ((conj (degree_co_wrt_tm_ind' H1 H2 H3 H4 H5 H6 H7 H8 H9 H10 H11 H12 H13 H14 H15 H16 H17 H18 H19 H20 H21 H22 H23 H24 H25 H26 H27 H28 H29 H30 H31 H32 H33 H34 H35 H36 H37 H38 H39 H40 H41 H42 H43 H44 H45 H46 H47 H48 H49 H50 H51 H52 H53)
-  (degree_constraint_wrt_tm_ind' H1 H2 H3 H4 H5 H6 H7 H8 H9 H10 H11 H12 H13 H14 H15 H16 H17 H18 H19 H20 H21 H22 H23 H24 H25 H26 H27 H28 H29 H30 H31 H32 H33 H34 H35 H36 H37 H38 H39 H40 H41 H42 H43 H44 H45 H46 H47 H48 H49 H50 H51 H52 H53)))))).
+  fun H1 H2 H3 H4 H5 H6 H7 H8 H9 H10 H11 H12 H13 H14 H15 H16 H17 H18 H19 H20 H21 H22 H23 H24 H25 H26 H27 H28 H29 H30 H31 H32 H33 H34 H35 H36 H37 H38 H39 H40 H41 H42 H43 H44 H45 H46 H47 H48 H49 H50 H51 H52 =>
+  (conj (degree_tm_wrt_tm_ind' H1 H2 H3 H4 H5 H6 H7 H8 H9 H10 H11 H12 H13 H14 H15 H16 H17 H18 H19 H20 H21 H22 H23 H24 H25 H26 H27 H28 H29 H30 H31 H32 H33 H34 H35 H36 H37 H38 H39 H40 H41 H42 H43 H44 H45 H46 H47 H48 H49 H50 H51 H52)
+  ((conj (degree_brs_wrt_tm_ind' H1 H2 H3 H4 H5 H6 H7 H8 H9 H10 H11 H12 H13 H14 H15 H16 H17 H18 H19 H20 H21 H22 H23 H24 H25 H26 H27 H28 H29 H30 H31 H32 H33 H34 H35 H36 H37 H38 H39 H40 H41 H42 H43 H44 H45 H46 H47 H48 H49 H50 H51 H52)
+  ((conj (degree_co_wrt_tm_ind' H1 H2 H3 H4 H5 H6 H7 H8 H9 H10 H11 H12 H13 H14 H15 H16 H17 H18 H19 H20 H21 H22 H23 H24 H25 H26 H27 H28 H29 H30 H31 H32 H33 H34 H35 H36 H37 H38 H39 H40 H41 H42 H43 H44 H45 H46 H47 H48 H49 H50 H51 H52)
+  (degree_constraint_wrt_tm_ind' H1 H2 H3 H4 H5 H6 H7 H8 H9 H10 H11 H12 H13 H14 H15 H16 H17 H18 H19 H20 H21 H22 H23 H24 H25 H26 H27 H28 H29 H30 H31 H32 H33 H34 H35 H36 H37 H38 H39 H40 H41 H42 H43 H44 H45 H46 H47 H48 H49 H50 H51 H52)))))).
 
 Scheme degree_tm_wrt_co_ind' := Induction for degree_tm_wrt_co Sort Prop
   with degree_brs_wrt_co_ind' := Induction for degree_brs_wrt_co Sort Prop
@@ -733,11 +744,11 @@ Scheme degree_tm_wrt_co_ind' := Induction for degree_tm_wrt_co Sort Prop
   with degree_constraint_wrt_co_ind' := Induction for degree_constraint_wrt_co Sort Prop.
 
 Definition degree_tm_wrt_co_degree_brs_wrt_co_degree_co_wrt_co_degree_constraint_wrt_co_mutind :=
-  fun H1 H2 H3 H4 H5 H6 H7 H8 H9 H10 H11 H12 H13 H14 H15 H16 H17 H18 H19 H20 H21 H22 H23 H24 H25 H26 H27 H28 H29 H30 H31 H32 H33 H34 H35 H36 H37 H38 H39 H40 H41 H42 H43 H44 H45 H46 H47 H48 H49 H50 H51 H52 H53 =>
-  (conj (degree_tm_wrt_co_ind' H1 H2 H3 H4 H5 H6 H7 H8 H9 H10 H11 H12 H13 H14 H15 H16 H17 H18 H19 H20 H21 H22 H23 H24 H25 H26 H27 H28 H29 H30 H31 H32 H33 H34 H35 H36 H37 H38 H39 H40 H41 H42 H43 H44 H45 H46 H47 H48 H49 H50 H51 H52 H53)
-  ((conj (degree_brs_wrt_co_ind' H1 H2 H3 H4 H5 H6 H7 H8 H9 H10 H11 H12 H13 H14 H15 H16 H17 H18 H19 H20 H21 H22 H23 H24 H25 H26 H27 H28 H29 H30 H31 H32 H33 H34 H35 H36 H37 H38 H39 H40 H41 H42 H43 H44 H45 H46 H47 H48 H49 H50 H51 H52 H53)
-  ((conj (degree_co_wrt_co_ind' H1 H2 H3 H4 H5 H6 H7 H8 H9 H10 H11 H12 H13 H14 H15 H16 H17 H18 H19 H20 H21 H22 H23 H24 H25 H26 H27 H28 H29 H30 H31 H32 H33 H34 H35 H36 H37 H38 H39 H40 H41 H42 H43 H44 H45 H46 H47 H48 H49 H50 H51 H52 H53)
-  (degree_constraint_wrt_co_ind' H1 H2 H3 H4 H5 H6 H7 H8 H9 H10 H11 H12 H13 H14 H15 H16 H17 H18 H19 H20 H21 H22 H23 H24 H25 H26 H27 H28 H29 H30 H31 H32 H33 H34 H35 H36 H37 H38 H39 H40 H41 H42 H43 H44 H45 H46 H47 H48 H49 H50 H51 H52 H53)))))).
+  fun H1 H2 H3 H4 H5 H6 H7 H8 H9 H10 H11 H12 H13 H14 H15 H16 H17 H18 H19 H20 H21 H22 H23 H24 H25 H26 H27 H28 H29 H30 H31 H32 H33 H34 H35 H36 H37 H38 H39 H40 H41 H42 H43 H44 H45 H46 H47 H48 H49 H50 H51 H52 =>
+  (conj (degree_tm_wrt_co_ind' H1 H2 H3 H4 H5 H6 H7 H8 H9 H10 H11 H12 H13 H14 H15 H16 H17 H18 H19 H20 H21 H22 H23 H24 H25 H26 H27 H28 H29 H30 H31 H32 H33 H34 H35 H36 H37 H38 H39 H40 H41 H42 H43 H44 H45 H46 H47 H48 H49 H50 H51 H52)
+  ((conj (degree_brs_wrt_co_ind' H1 H2 H3 H4 H5 H6 H7 H8 H9 H10 H11 H12 H13 H14 H15 H16 H17 H18 H19 H20 H21 H22 H23 H24 H25 H26 H27 H28 H29 H30 H31 H32 H33 H34 H35 H36 H37 H38 H39 H40 H41 H42 H43 H44 H45 H46 H47 H48 H49 H50 H51 H52)
+  ((conj (degree_co_wrt_co_ind' H1 H2 H3 H4 H5 H6 H7 H8 H9 H10 H11 H12 H13 H14 H15 H16 H17 H18 H19 H20 H21 H22 H23 H24 H25 H26 H27 H28 H29 H30 H31 H32 H33 H34 H35 H36 H37 H38 H39 H40 H41 H42 H43 H44 H45 H46 H47 H48 H49 H50 H51 H52)
+  (degree_constraint_wrt_co_ind' H1 H2 H3 H4 H5 H6 H7 H8 H9 H10 H11 H12 H13 H14 H15 H16 H17 H18 H19 H20 H21 H22 H23 H24 H25 H26 H27 H28 H29 H30 H31 H32 H33 H34 H35 H36 H37 H38 H39 H40 H41 H42 H43 H44 H45 H46 H47 H48 H49 H50 H51 H52)))))).
 
 Hint Constructors degree_tm_wrt_tm : core lngen.
 
@@ -760,8 +771,6 @@ Hint Constructors degree_constraint_wrt_co : core lngen.
 (** * Local closure (version in [Set], induction principles) *)
 
 Inductive lc_set_tm : tm -> Set :=
-  | lc_set_a_Star :
-    lc_set_tm (a_Star)
   | lc_set_a_Var_f : forall x1,
     lc_set_tm (a_Var_f x1)
   | lc_set_a_Abs : forall rho1 A1 b1,
@@ -941,11 +950,11 @@ Scheme lc_tm_ind' := Induction for lc_tm Sort Prop
   with lc_constraint_ind' := Induction for lc_constraint Sort Prop.
 
 Definition lc_tm_lc_brs_lc_co_lc_constraint_mutind :=
-  fun H1 H2 H3 H4 H5 H6 H7 H8 H9 H10 H11 H12 H13 H14 H15 H16 H17 H18 H19 H20 H21 H22 H23 H24 H25 H26 H27 H28 H29 H30 H31 H32 H33 H34 H35 H36 H37 H38 H39 H40 H41 H42 H43 H44 H45 H46 H47 H48 H49 H50 H51 =>
-  (conj (lc_tm_ind' H1 H2 H3 H4 H5 H6 H7 H8 H9 H10 H11 H12 H13 H14 H15 H16 H17 H18 H19 H20 H21 H22 H23 H24 H25 H26 H27 H28 H29 H30 H31 H32 H33 H34 H35 H36 H37 H38 H39 H40 H41 H42 H43 H44 H45 H46 H47 H48 H49 H50 H51)
-  ((conj (lc_brs_ind' H1 H2 H3 H4 H5 H6 H7 H8 H9 H10 H11 H12 H13 H14 H15 H16 H17 H18 H19 H20 H21 H22 H23 H24 H25 H26 H27 H28 H29 H30 H31 H32 H33 H34 H35 H36 H37 H38 H39 H40 H41 H42 H43 H44 H45 H46 H47 H48 H49 H50 H51)
-  ((conj (lc_co_ind' H1 H2 H3 H4 H5 H6 H7 H8 H9 H10 H11 H12 H13 H14 H15 H16 H17 H18 H19 H20 H21 H22 H23 H24 H25 H26 H27 H28 H29 H30 H31 H32 H33 H34 H35 H36 H37 H38 H39 H40 H41 H42 H43 H44 H45 H46 H47 H48 H49 H50 H51)
-  (lc_constraint_ind' H1 H2 H3 H4 H5 H6 H7 H8 H9 H10 H11 H12 H13 H14 H15 H16 H17 H18 H19 H20 H21 H22 H23 H24 H25 H26 H27 H28 H29 H30 H31 H32 H33 H34 H35 H36 H37 H38 H39 H40 H41 H42 H43 H44 H45 H46 H47 H48 H49 H50 H51)))))).
+  fun H1 H2 H3 H4 H5 H6 H7 H8 H9 H10 H11 H12 H13 H14 H15 H16 H17 H18 H19 H20 H21 H22 H23 H24 H25 H26 H27 H28 H29 H30 H31 H32 H33 H34 H35 H36 H37 H38 H39 H40 H41 H42 H43 H44 H45 H46 H47 H48 H49 H50 =>
+  (conj (lc_tm_ind' H1 H2 H3 H4 H5 H6 H7 H8 H9 H10 H11 H12 H13 H14 H15 H16 H17 H18 H19 H20 H21 H22 H23 H24 H25 H26 H27 H28 H29 H30 H31 H32 H33 H34 H35 H36 H37 H38 H39 H40 H41 H42 H43 H44 H45 H46 H47 H48 H49 H50)
+  ((conj (lc_brs_ind' H1 H2 H3 H4 H5 H6 H7 H8 H9 H10 H11 H12 H13 H14 H15 H16 H17 H18 H19 H20 H21 H22 H23 H24 H25 H26 H27 H28 H29 H30 H31 H32 H33 H34 H35 H36 H37 H38 H39 H40 H41 H42 H43 H44 H45 H46 H47 H48 H49 H50)
+  ((conj (lc_co_ind' H1 H2 H3 H4 H5 H6 H7 H8 H9 H10 H11 H12 H13 H14 H15 H16 H17 H18 H19 H20 H21 H22 H23 H24 H25 H26 H27 H28 H29 H30 H31 H32 H33 H34 H35 H36 H37 H38 H39 H40 H41 H42 H43 H44 H45 H46 H47 H48 H49 H50)
+  (lc_constraint_ind' H1 H2 H3 H4 H5 H6 H7 H8 H9 H10 H11 H12 H13 H14 H15 H16 H17 H18 H19 H20 H21 H22 H23 H24 H25 H26 H27 H28 H29 H30 H31 H32 H33 H34 H35 H36 H37 H38 H39 H40 H41 H42 H43 H44 H45 H46 H47 H48 H49 H50)))))).
 
 Scheme lc_set_tm_ind' := Induction for lc_set_tm Sort Prop
   with lc_set_brs_ind' := Induction for lc_set_brs Sort Prop
@@ -953,11 +962,11 @@ Scheme lc_set_tm_ind' := Induction for lc_set_tm Sort Prop
   with lc_set_constraint_ind' := Induction for lc_set_constraint Sort Prop.
 
 Definition lc_set_tm_lc_set_brs_lc_set_co_lc_set_constraint_mutind :=
-  fun H1 H2 H3 H4 H5 H6 H7 H8 H9 H10 H11 H12 H13 H14 H15 H16 H17 H18 H19 H20 H21 H22 H23 H24 H25 H26 H27 H28 H29 H30 H31 H32 H33 H34 H35 H36 H37 H38 H39 H40 H41 H42 H43 H44 H45 H46 H47 H48 H49 H50 H51 =>
-  (conj (lc_set_tm_ind' H1 H2 H3 H4 H5 H6 H7 H8 H9 H10 H11 H12 H13 H14 H15 H16 H17 H18 H19 H20 H21 H22 H23 H24 H25 H26 H27 H28 H29 H30 H31 H32 H33 H34 H35 H36 H37 H38 H39 H40 H41 H42 H43 H44 H45 H46 H47 H48 H49 H50 H51)
-  ((conj (lc_set_brs_ind' H1 H2 H3 H4 H5 H6 H7 H8 H9 H10 H11 H12 H13 H14 H15 H16 H17 H18 H19 H20 H21 H22 H23 H24 H25 H26 H27 H28 H29 H30 H31 H32 H33 H34 H35 H36 H37 H38 H39 H40 H41 H42 H43 H44 H45 H46 H47 H48 H49 H50 H51)
-  ((conj (lc_set_co_ind' H1 H2 H3 H4 H5 H6 H7 H8 H9 H10 H11 H12 H13 H14 H15 H16 H17 H18 H19 H20 H21 H22 H23 H24 H25 H26 H27 H28 H29 H30 H31 H32 H33 H34 H35 H36 H37 H38 H39 H40 H41 H42 H43 H44 H45 H46 H47 H48 H49 H50 H51)
-  (lc_set_constraint_ind' H1 H2 H3 H4 H5 H6 H7 H8 H9 H10 H11 H12 H13 H14 H15 H16 H17 H18 H19 H20 H21 H22 H23 H24 H25 H26 H27 H28 H29 H30 H31 H32 H33 H34 H35 H36 H37 H38 H39 H40 H41 H42 H43 H44 H45 H46 H47 H48 H49 H50 H51)))))).
+  fun H1 H2 H3 H4 H5 H6 H7 H8 H9 H10 H11 H12 H13 H14 H15 H16 H17 H18 H19 H20 H21 H22 H23 H24 H25 H26 H27 H28 H29 H30 H31 H32 H33 H34 H35 H36 H37 H38 H39 H40 H41 H42 H43 H44 H45 H46 H47 H48 H49 H50 =>
+  (conj (lc_set_tm_ind' H1 H2 H3 H4 H5 H6 H7 H8 H9 H10 H11 H12 H13 H14 H15 H16 H17 H18 H19 H20 H21 H22 H23 H24 H25 H26 H27 H28 H29 H30 H31 H32 H33 H34 H35 H36 H37 H38 H39 H40 H41 H42 H43 H44 H45 H46 H47 H48 H49 H50)
+  ((conj (lc_set_brs_ind' H1 H2 H3 H4 H5 H6 H7 H8 H9 H10 H11 H12 H13 H14 H15 H16 H17 H18 H19 H20 H21 H22 H23 H24 H25 H26 H27 H28 H29 H30 H31 H32 H33 H34 H35 H36 H37 H38 H39 H40 H41 H42 H43 H44 H45 H46 H47 H48 H49 H50)
+  ((conj (lc_set_co_ind' H1 H2 H3 H4 H5 H6 H7 H8 H9 H10 H11 H12 H13 H14 H15 H16 H17 H18 H19 H20 H21 H22 H23 H24 H25 H26 H27 H28 H29 H30 H31 H32 H33 H34 H35 H36 H37 H38 H39 H40 H41 H42 H43 H44 H45 H46 H47 H48 H49 H50)
+  (lc_set_constraint_ind' H1 H2 H3 H4 H5 H6 H7 H8 H9 H10 H11 H12 H13 H14 H15 H16 H17 H18 H19 H20 H21 H22 H23 H24 H25 H26 H27 H28 H29 H30 H31 H32 H33 H34 H35 H36 H37 H38 H39 H40 H41 H42 H43 H44 H45 H46 H47 H48 H49 H50)))))).
 
 Scheme lc_set_tm_rec' := Induction for lc_set_tm Sort Set
   with lc_set_brs_rec' := Induction for lc_set_brs Sort Set
@@ -965,11 +974,11 @@ Scheme lc_set_tm_rec' := Induction for lc_set_tm Sort Set
   with lc_set_constraint_rec' := Induction for lc_set_constraint Sort Set.
 
 Definition lc_set_tm_lc_set_brs_lc_set_co_lc_set_constraint_mutrec :=
-  fun H1 H2 H3 H4 H5 H6 H7 H8 H9 H10 H11 H12 H13 H14 H15 H16 H17 H18 H19 H20 H21 H22 H23 H24 H25 H26 H27 H28 H29 H30 H31 H32 H33 H34 H35 H36 H37 H38 H39 H40 H41 H42 H43 H44 H45 H46 H47 H48 H49 H50 H51 =>
-  (pair ((pair ((pair (lc_set_tm_rec' H1 H2 H3 H4 H5 H6 H7 H8 H9 H10 H11 H12 H13 H14 H15 H16 H17 H18 H19 H20 H21 H22 H23 H24 H25 H26 H27 H28 H29 H30 H31 H32 H33 H34 H35 H36 H37 H38 H39 H40 H41 H42 H43 H44 H45 H46 H47 H48 H49 H50 H51)
-  (lc_set_brs_rec' H1 H2 H3 H4 H5 H6 H7 H8 H9 H10 H11 H12 H13 H14 H15 H16 H17 H18 H19 H20 H21 H22 H23 H24 H25 H26 H27 H28 H29 H30 H31 H32 H33 H34 H35 H36 H37 H38 H39 H40 H41 H42 H43 H44 H45 H46 H47 H48 H49 H50 H51)))
-  (lc_set_co_rec' H1 H2 H3 H4 H5 H6 H7 H8 H9 H10 H11 H12 H13 H14 H15 H16 H17 H18 H19 H20 H21 H22 H23 H24 H25 H26 H27 H28 H29 H30 H31 H32 H33 H34 H35 H36 H37 H38 H39 H40 H41 H42 H43 H44 H45 H46 H47 H48 H49 H50 H51)))
-  (lc_set_constraint_rec' H1 H2 H3 H4 H5 H6 H7 H8 H9 H10 H11 H12 H13 H14 H15 H16 H17 H18 H19 H20 H21 H22 H23 H24 H25 H26 H27 H28 H29 H30 H31 H32 H33 H34 H35 H36 H37 H38 H39 H40 H41 H42 H43 H44 H45 H46 H47 H48 H49 H50 H51)).
+  fun H1 H2 H3 H4 H5 H6 H7 H8 H9 H10 H11 H12 H13 H14 H15 H16 H17 H18 H19 H20 H21 H22 H23 H24 H25 H26 H27 H28 H29 H30 H31 H32 H33 H34 H35 H36 H37 H38 H39 H40 H41 H42 H43 H44 H45 H46 H47 H48 H49 H50 =>
+  (pair ((pair ((pair (lc_set_tm_rec' H1 H2 H3 H4 H5 H6 H7 H8 H9 H10 H11 H12 H13 H14 H15 H16 H17 H18 H19 H20 H21 H22 H23 H24 H25 H26 H27 H28 H29 H30 H31 H32 H33 H34 H35 H36 H37 H38 H39 H40 H41 H42 H43 H44 H45 H46 H47 H48 H49 H50)
+  (lc_set_brs_rec' H1 H2 H3 H4 H5 H6 H7 H8 H9 H10 H11 H12 H13 H14 H15 H16 H17 H18 H19 H20 H21 H22 H23 H24 H25 H26 H27 H28 H29 H30 H31 H32 H33 H34 H35 H36 H37 H38 H39 H40 H41 H42 H43 H44 H45 H46 H47 H48 H49 H50)))
+  (lc_set_co_rec' H1 H2 H3 H4 H5 H6 H7 H8 H9 H10 H11 H12 H13 H14 H15 H16 H17 H18 H19 H20 H21 H22 H23 H24 H25 H26 H27 H28 H29 H30 H31 H32 H33 H34 H35 H36 H37 H38 H39 H40 H41 H42 H43 H44 H45 H46 H47 H48 H49 H50)))
+  (lc_set_constraint_rec' H1 H2 H3 H4 H5 H6 H7 H8 H9 H10 H11 H12 H13 H14 H15 H16 H17 H18 H19 H20 H21 H22 H23 H24 H25 H26 H27 H28 H29 H30 H31 H32 H33 H34 H35 H36 H37 H38 H39 H40 H41 H42 H43 H44 H45 H46 H47 H48 H49 H50)).
 
 Hint Constructors lc_tm : core lngen.
 
@@ -1088,6 +1097,20 @@ forall nu1, 1 <= size_appflag nu1.
 Proof. Admitted.
 
 Hint Resolve size_appflag_min : lngen.
+
+(* begin hide *)
+
+Lemma size_F_min_mutual :
+(forall F1, 1 <= size_F F1).
+Proof. Admitted.
+
+(* end hide *)
+
+Lemma size_F_min :
+forall F1, 1 <= size_F F1.
+Proof. Admitted.
+
+Hint Resolve size_F_min : lngen.
 
 (* begin hide *)
 
@@ -4552,6 +4575,12 @@ Ltac role_lc_exists_tac :=
           end).
 
 Ltac appflag_lc_exists_tac :=
+  repeat (match goal with
+            | H : _ |- _ =>
+              fail 1
+          end).
+
+Ltac F_lc_exists_tac :=
   repeat (match goal with
             | H : _ |- _ =>
               fail 1
